Fix AArch64.TakeException proof
Add lemmas for the exception case of writing PCC, and add a proof and a
register accessibility assumption to the AArch64.TakeException lemma.
The latter leads to additional register accessibility conditions for
other lemmas.  This patch adds those for the manually patched functions.
For functions and instructions with loops, a register accessibility loop
invariant may now be required; it should be possible to handle this
automatically in the traces_enabledI tactic.

CHERI_Instantiation.thy
@@ -898,8 +898,11 @@ definition instr_raises_ex :: "instr \<Rightarrow> register_value trace \<Righta
 definition fetch_raises_ex :: "register_value trace \<Rightarrow> bool" where
   "fetch_raises_ex t \<equiv> hasException t instr_fetch"
 
+text \<open>Over-approximation of allowed exception targets
+TODO: Restrict to valid branch targets of KCC caps with (small) offset?\<close>
+
 definition exception_targets :: "register_value set \<Rightarrow> Capability set" where
-  "exception_targets rvs \<equiv> \<Union>(caps_of_regval ` rvs)"
+  "exception_targets rvs \<equiv> derivable (\<Union>(caps_of_regval ` rvs))"
 
 fun acctype_of_AccType :: "AccType \<Rightarrow> bool \<Rightarrow> acctype" where
   "acctype_of_AccType AccType_PTW _ = PTW"
@@ -955,6 +958,7 @@ lemma ISA_simps[simp]:
   "isa.instr_fetch ISA = instr_fetch"
   "isa.caps_of_regval ISA = caps_of_regval"
   "isa.is_translation_event ISA = is_translation_event"
+  "isa.exception_targets ISA = exception_targets"
   by (auto simp: ISA_def)
 
 lemma no_cap_regvals[simp]:
@@ -1549,10 +1553,10 @@ lemma update_subrange_addr_CapWithTagClear_derivable:
 
 lemma update_subrange_addr_CapIsRepresentable_derivable:
   assumes "Run (CapIsRepresentable c addr) t a" and "a"
-    and "c \<in> derivable_caps s"
+    and "c \<in> derivable C"
     and "CapIsTagSet c \<longrightarrow> \<not>CapIsSealed c"
-  shows "update_subrange_vec_dec c CAP_VALUE_HI_BIT CAP_VALUE_LO_BIT addr \<in> derivable_caps s"
-    (is "?c' \<in> derivable_caps s")
+  shows "update_subrange_vec_dec c CAP_VALUE_HI_BIT CAP_VALUE_LO_BIT addr \<in> derivable C"
+    (is "?c' \<in> derivable C")
 proof -
   have "get_base ?c' = get_base c" and "get_limit ?c' = get_limit c"
     using assms(1-2)
@@ -1572,11 +1576,17 @@ proof -
     using assms(4)
     unfolding derivable_caps_def
     by (auto simp: leq_cap_def)
-  from derivable.Restrict[OF _ this]
-  show ?thesis
-    using assms(3) tag
-    by (auto simp: derivable_caps_def)
+  from derivable.Restrict[OF assms(3) this]
+  show ?thesis .
 qed
+
+lemma update_subrange_addr_CapIsRepresentable_derivable_caps:
+  assumes "Run (CapIsRepresentable c addr) t a" and "a"
+    and "c \<in> derivable_caps s"
+    and "CapIsTagSet c \<longrightarrow> \<not>CapIsSealed c"
+  shows "update_subrange_vec_dec c CAP_VALUE_HI_BIT CAP_VALUE_LO_BIT addr \<in> derivable_caps s"
+  using assms update_subrange_addr_CapIsRepresentable_derivable[OF assms(1,2)]
+  by (auto simp: derivable_caps_def update_subrange_vec_dec_test_bit)
 
 lemmas update_subrange_if_derivable =
   if_split[where P = "\<lambda>c. update_subrange_vec_dec c hi lo v \<in> derivable_caps s" for hi lo v s, THEN iffD2]
@@ -1992,6 +2002,12 @@ next
     by (auto simp: leq_cap_def)
 qed
 
+lemma branch_caps_derivable:
+  assumes "c' \<in> branch_caps c" and "CapIsTagSet c \<longrightarrow> \<not>CapIsSealed c" and "c \<in> derivable C"
+  shows "c' \<in> derivable C"
+  using branch_caps_leq[OF assms(1,2)] assms(3)
+  by (auto intro: derivable.Restrict)
+
 lemma branch_caps_128th_iff:
   assumes "c' \<in> branch_caps c"
   shows "c' !! 128 \<longleftrightarrow> c !! 128"
@@ -2001,8 +2017,8 @@ lemma branch_caps_128th_iff:
 lemma branch_caps_derivable_caps:
   assumes "c' \<in> branch_caps c" and "c \<in> derivable_caps s" and "CapIsTagSet c \<longrightarrow> \<not>CapIsSealed c"
   shows "c' \<in> derivable_caps s"
-  using assms(2) branch_caps_leq[OF assms(1,3)] branch_caps_128th_iff[OF assms(1)]
-  by (auto simp: derivable_caps_def intro: derivable.Restrict)
+  using assms(2) branch_caps_derivable[OF assms(1,3)] branch_caps_128th_iff[OF assms(1)]
+  by (auto simp: derivable_caps_def)
 
 lemma CapSetFlags_mask_56_normalise_cursor_flags:
   "CapSetFlags c (CapGetValue c AND mask 56) = normalise_cursor_flags c False"
